general hindsight reasoning

templates/hindsight/hindsight.v
@@ -13,18 +13,6 @@ Set Default Proof Using "All".
 From iris.bi.lib Require Import fractional.
 Require Export one_shot_proph typed_proph.
 
-(*
-Parameter search : val.
-Parameter insert : val.
-Parameter delete : val.
-
-Definition ssOp : val :=
-  λ: "OP" "r",     
-    if: "OP" = #0 then search "r"
-    else if: "OP" = #1 then insert "r"
-    else delete "r".
-*)
-
 Parameter dsOp : val.
 
 Definition dsOp' : val :=
@@ -42,19 +30,79 @@ Section Proof.
   (* Data structure specific definitions *)
 
   Parameter Op : Type.
-  Parameter snapshot : Type.
-  Parameter snapshotUR : ucmra.
-  Parameter test : snapshot -> snapshotUR.
-  Coercion test : snapshot >-> snapshotUR.
   Parameter Op_to_val : Op -> val.
-  Parameter absT : Type.
+
+  Parameter snapshotUR : ucmra.
+  Definition snapshot := ucmra_car snapshotUR.
+
   Parameter absTUR : ucmra.
+  Definition absT := ucmra_car absTUR.
+
   Parameter resT : Type.
+  Parameter resT_to_base_lit : resT -> base_lit.
+  Coercion resT_to_base_lit : resT >-> base_lit.
+  Parameter resT_from_val : val -> option resT.
+  Parameter resT_to_val : resT -> val.
+  Parameter resT_inj_prop : ∀ (r : resT), resT_from_val (resT_to_val r) = Some r.
+  Definition resTProph : TypedProphSpec :=
+    mkTypedProphSpec resT resT_from_val resT_to_val resT_inj_prop.
+  Definition resTTypedProph `{!heapGS Σ} := make_TypedProph resTProph.
+  Parameter resT_proph_resolve : ∀ (res: resT), resT_from_val #res = Some res.
+  
   Parameter seq_spec : Op -> absT -> absT -> resT -> Prop.
   Parameter abs : snapshot -> absT.
   Parameter updater_thread: Op -> resT -> bool.
 
-  Parameter seq_spec_dec : ∀ op s s' res, Decision (seq_spec op s s' res).
+  Parameter neg_seq_spec_dec : ∀ op c c' res, Decision (¬ seq_spec op c c' res).
+  Parameter seq_spec_dec : ∀ op c c' res, Decision (seq_spec op c c' res).
+  Parameter updater_thread_dec: ∀ op res b, Decision (updater_thread op res = b).  
+  
+  Parameter snapshotUR_discrete : CmraDiscrete snapshotUR.
+  Parameter absTUR_discrete : CmraDiscrete absTUR.
+  Parameter snapshot_leibnizequiv : LeibnizEquiv (snapshot).
+  Parameter snapshot_lookuptotal : LookupTotal nat snapshot (gmap nat snapshot).
+  Parameter snapshot_inhabited : Inhabited snapshot.
+  Parameter resT_inhabited : Inhabited resT.
+  Parameter Op_inhabited : Inhabited Op.
+
+  Instance snapshotUR_discrete' : CmraDiscrete snapshotUR.
+  Proof.
+    apply snapshotUR_discrete.
+  Qed.
+  
+  Instance absTUR_discrete' : CmraDiscrete absTUR.
+  Proof.
+    apply absTUR_discrete.
+  Qed.
+
+  Instance snapshot_leibnizequiv' : LeibnizEquiv (snapshot).
+  Proof.
+    apply snapshot_leibnizequiv.
+  Qed.  
+  
+  Instance snapshot_lookuptotal' : LookupTotal nat snapshot (gmap nat snapshot).
+  Proof.
+    apply snapshot_lookuptotal.
+  Qed.
+
+  Instance snapshot_inhabited' : Inhabited snapshot.
+  Proof.
+    apply snapshot_inhabited.
+  Qed.
+
+  Instance resT_inhabited' : Inhabited resT.
+  Proof.
+    apply resT_inhabited.
+  Qed.
+
+  Instance Op_inhabited' : Inhabited Op.
+  Proof.
+    apply Op_inhabited.
+  Qed.
+
+
+
+  
   (* Parameter snapshot_eq: EqDecision snapshot.*)
   
   (* RAs used in proof *)
@@ -62,10 +110,10 @@ Section Proof.
   Definition auth_natUR := authUR $ max_natUR.
   Definition agree_snapshotR := agreeR $ snapshotUR.
   Definition frac_absTR := dfrac_agreeR $ absTUR.
-  Definition historyR := gmapUR nat $ agree_snapshotR.
-  Definition auth_historyR := authR $ historyR.
-  Definition tokenUR := exclR unitO.
+  Definition historyR := gmapUR nat $ snapshotUR.
+  Definition auth_historyR := authR $ gmapUR nat $ agree_snapshotR.
   Definition frac_historyR := dfrac_agreeR $ historyR.
+  Definition tokenUR := exclR unitO.
   Definition set_tidR := authR (gsetUR proph_id). 
   Definition thread_viewR := authUR $ 
                               gmapUR proph_id $ 
@@ -92,50 +140,31 @@ Section Proof.
   
   Instance subG_dsΣ {Σ} : subG dsΣ Σ → dsG Σ.
   Proof. solve_inG. Qed.
-End Proof.
 
-Section counter.
-  Context (snapshotUR : ucmra) (absTUR: ucmra).
-  Context {Σ} `{!heapGS Σ, !dsG snapshotUR absTUR Σ}.
+  Context {Σ} `{!heapGS Σ, !dsG Σ}.
   Notation iProp := (iProp Σ).
   Implicit Types M : gmap nat snapshot.
   Implicit Types T : nat.
-
+  
   Global Definition cntrN N := N .@ "cntr".
   Global Definition threadN N := N .@ "thread".
-
-  Instance snapshot_lookuptotal : LookupTotal nat snapshotUR (gmap nat snapshot).
-  Proof.
-  Admitted.
+  
 
   Definition map_max (M: gmap nat snapshot) : nat := 
     max_list (elements (dom M)).
 
-  Definition hist γ_t γ_m M T (s: snapshot) : iProp :=
+  Definition hist γ_t γ_m M T : iProp :=
     ∃ (M': gmap nat (agreeR (_))),
       own γ_t (● MaxNat T) ∗ own γ_m (● M')
     ∗ ⌜T = map_max M⌝
     ∗ ⌜map_Forall (λ k a, a = to_agree (M !!! k)) M'⌝
     ∗ ⌜∀ t, t < T → M !!! t ≠ M !!! (t+1)%nat⌝.
   
-  Definition dsRep γ_r (a: absTUR) : iProp := 
-    own γ_r (to_frac_agree (1/2) a).
+  Definition dsRep γ_s (a: absTUR) : iProp := 
+    own γ_s (to_frac_agree (1/2) a).
 
-  Definition dsRepI γ_r (a: absTUR) : iProp := 
-    own γ_r (to_frac_agree (1/2) a).
-
-(*  
-  Definition per_tick_inv (t: nat) : iProp := True. 
-    
-  Definition transition_inv (M: gmap nat nat) (T: nat) : iProp :=
-    ⌜∀ (t1 t2: nat) (v: nat), t1 ≤ t2 → 
-                                M !!! t1 ≤ v ≤ M !!! t2 → 
-                                  ∃ (t: nat), t1 ≤ t ≤ t2 ∧ M !!! t = v⌝.
-  
-  Definition resources γ_l1 γ_l2 l1 l2 (n1 n2 n: nat) : iProp :=
-    l1 ↦ #n1 ∗ l2 ↦ #n2 ∗ ⌜(n1 + n2 = n)%nat⌝
-    ∗ own γ_l1 (● MaxNat n1) ∗ own γ_l2 (● MaxNat n2).
-*)
+  Definition dsRepI γ_s (a: absTUR) : iProp := 
+    own γ_s (to_frac_agree (1/2) a).
     
   (** Helping Inv **)
   
@@ -169,7 +198,7 @@ Section counter.
   Definition Pending (P: iProp) M T op vp t0 : iProp := 
     P ∗ £1 ∗ ¬ past_lin M T op vp t0.
 
-  Definition Done γ_tk (Q: val → iProp) M T op (vp: nat) t0 : iProp := 
+  Definition Done γ_tk (Q: val → iProp) M T op (vp: resT) t0 : iProp := 
       (Q #vp ∨ own γ_tk (Excl ())) ∗ past_lin M T op vp t0.
 
   Definition State γ_sy γ_tk P Q M T op vp t0 : iProp :=
@@ -181,7 +210,7 @@ Section counter.
     own γ_ght (◯ {[t_id := to_agree (t0, γ_sy)]}) ∗ own γ_t (◯ MaxNat t0).
 
   Definition Reg N γ_t γ_s γ_ght t_id M : iProp :=
-    ∃ γ_tk γ_sy Q op (vp t0: nat) (vtid: val), 
+    ∃ γ_tk γ_sy Q op vp t0 (vtid: val), 
         proph1 t_id vtid
       ∗ thread_vars γ_t γ_ght γ_sy t_id t0
       ∗ own (γ_sy) (to_frac_agree (1/2) M)
@@ -195,84 +224,51 @@ Section counter.
   
   Definition ds_inv N γ_t γ_s γ_m γ_td γ_ght template_inv : iProp :=
     inv (cntrN N)
-    (∃ M T n,
-      cntr γ_s n ∗ ⌜abs (M !!! T) = n⌝
+    (∃ M T (s: snapshot),
+      dsRepI γ_s (abs s) ∗ ⌜M !!! T = s⌝
     ∗ hist γ_t γ_m M T
     ∗ helping_inv N γ_t γ_s γ_td γ_ght M
-    ∗ template_inv M T).
-    
+    ∗ template_inv M T s).
+(*    
+  Instance dsRep_timeless : ∀ γ_s C, Timeless (dsRep γ_s C).
+  Proof.
+    intros γ_s C. rewrite /dsRep. Search Timeless. 
+    apply own_timeless; apply _.
+  Qed.   
+*)    
   Definition update_helping_protocol N γ_t γ_s γ_td γ_ght : iProp :=
-        ∀ M T n n1 n2, 
+        ∀ M T n s, 
           ⌜map_max M = T⌝ -∗   
-            cntr γ_s n -∗ own γ_t (● MaxNat T) -∗ 
+            dsRep γ_s n -∗ own γ_t (● MaxNat T) -∗ 
               helping_inv N γ_t γ_s γ_td γ_ght M ={⊤ ∖ ↑cntrN N}=∗
-                helping_inv N γ_t γ_s γ_td γ_ght (<[T := (n1, n2)]> M) 
-                ∗ cntr γ_s n ∗ own γ_t (● MaxNat T).
+                helping_inv N γ_t γ_s γ_td γ_ght (<[T := s]> M) 
+                ∗ dsRep γ_s n ∗ own γ_t (● MaxNat T).
 
-  (** Proofs *)    
+  (** Proofs *)
 
-(*
-  Lemma counterOp_spec N γ_s γ_t γ_m γ_td γ_ght template_inv op l1 l2 γ_sy t_id t0 :
-          ds_inv N γ_t γ_s γ_m γ_td γ_ght template_inv -∗
-            update_helping_protocol N γ_t γ_s γ_td γ_ght -∗
-              thread_vars γ_t γ_ght γ_sy t_id t0 -∗
-                <<< True >>> 
-                     counterOp (Op_to_val op) #l1 #l2 @ ↑(cntrN N)
-                <<< ∃∃ res, past_lin_witness γ_m op res t0, RET #res >>>.
-  Proof.
-  Admitted.
-*)
-
-  Lemma readOp_spec N γ_s γ_t γ_m γ_td γ_ght template_inv l1 l2 γ_sy t_id t0 :
+  Parameter dsOp_spec: ∀ N γ_s γ_t γ_m γ_td γ_ght template_inv op r γ_sy t_id t0,
           ds_inv N γ_t γ_s γ_m γ_td γ_ght template_inv -∗
             □ update_helping_protocol N γ_t γ_s γ_td γ_ght -∗
               thread_vars γ_t γ_ght γ_sy t_id t0 -∗
                 {{{ True }}} 
-                     read #l1 #l2
-                {{{ res, RET #res; past_lin_witness γ_m readOp res t0  }}}.
-  Proof.
-  Admitted.
-
-  Lemma incrOp_spec N γ_s γ_t γ_m γ_td γ_ght template_inv l1 l2 γ_sy t_id t0 :
-          ds_inv N γ_t γ_s γ_m γ_td γ_ght template_inv -∗
-            □ update_helping_protocol N γ_t γ_s γ_td γ_ght -∗
-              thread_vars γ_t γ_ght γ_sy t_id t0 -∗
-                {{{ True }}} 
-                     incr #l1 #l2
-                {{{ res, RET #res; past_lin_witness γ_m incrOp res t0  }}}.
-  Proof.
-  Admitted.
-
-
-  Lemma counterOp_spec N γ_s γ_t γ_m γ_td γ_ght template_inv op l1 l2 γ_sy t_id t0 :
-          ds_inv N γ_t γ_s γ_m γ_td γ_ght template_inv -∗
-            □ update_helping_protocol N γ_t γ_s γ_td γ_ght -∗
-              thread_vars γ_t γ_ght γ_sy t_id t0 -∗
-                {{{ True }}} 
-                     counterOp (Op_to_val op) #l1 #l2
+                     dsOp (Op_to_val op) #r
                 {{{ res, RET #res; past_lin_witness γ_m op res t0  }}}.
-  Proof.
-    iIntros "#HInv #Upd_help #Thr_vars". iIntros (Φ) "!# _ Hpost".
-    wp_lam. wp_pures. unfold Op_to_val; destruct op; wp_pures.
-    - wp_apply readOp_spec; try done.
-    - wp_apply incrOp_spec; try done.
-  Qed.
 
 
-  Lemma counterOp'_spec N γ_s γ_t γ_m γ_td γ_ght template_inv op l1 l2 :
+  Lemma dsOp'_spec N γ_s γ_t γ_m γ_td γ_ght template_inv op r :
           ds_inv N γ_t γ_s γ_m γ_td γ_ght template_inv -∗
-              <<< ∀∀ n, Cntr γ_s n >>> 
-                     counterOp' (Op_to_val op) #l1 #l2 @ ↑(cntrN N)
-              <<< ∃∃ n' res, Cntr γ_s n' ∗ ⌜seq_spec op n n' res⌝, RET #res >>>.
+              <<< ∀∀ a, dsRep γ_s a >>> 
+                     dsOp' (Op_to_val op) #r @ ↑(cntrN N)
+              <<< ∃∃ a' res, dsRep γ_s a' ∗ ⌜seq_spec op a a' res⌝, RET #res >>>.
   Proof.
     iIntros "#HInv" (Φ) "AU". wp_lam. 
     wp_pure credit:"Hc". wp_pures.
     wp_apply wp_new_proph1; try done.
     iIntros (tid vtid)"Htid". wp_pures.
-    wp_apply (typed_proph_wp_new_proph1 NatTypedProph); first done.
+    wp_apply (typed_proph_wp_new_proph1 resTTypedProph); first done.
     iIntros (vp p)"Hproph". wp_pures.
     iApply fupd_wp.
-    iInv "HInv" as (M0 T0 n0) "(>HCntr & >%Habs0 & >Hist & Help & Templ)". 
+    iInv "HInv" as (M0 T0 s0) "(>HCntr & >%Habs0 & >Hist & Help & Templ)". 
     iDestruct "Help" as (R hγt)"(>HR & >Hγt 
                                 & >Domm_hγt & Hstar_reg)".
     iAssert (▷ (⌜tid ∉ R⌝ 
@@ -283,10 +279,7 @@ Section counter.
       - iEval (rewrite (big_sepS_elem_of_acc _ (R) tid); 
                             last by eauto) in "Hstar_reg".
         iDestruct "Hstar_reg" as "(Hreg & Hstar_reg')".
-        (* Issue with op *)
-        (* iDestruct "Hreg" as (? ? ? ? ? ? ?)"(H' & _)". *)
-        iAssert (∃ vtid', proph1 tid vtid')%I as (?)"H'".
-        { admit. }
+        iDestruct "Hreg" as (? ? ? ? ? ? ?)"(H' & _)".
         iAssert (▷ False)%I with "[H' Htid]" as "HF".
         iApply (proph1_exclusive tid with "[Htid]"); try done.
         iNext. iExFalso; try done.
@@ -324,11 +317,18 @@ Section counter.
     assert (map_max M0 = T0) as M_max. { admit. }
     iAssert (own γ_t (◯ (MaxNat T0))) as "HfragT0".
     { admit. }
+    
+    assert (∀ op c res, Decision (updater_thread op res = true 
+              ∨ (updater_thread op res = false 
+                  ∧ ¬ seq_spec op c c res))) as Hdec.
+    { intros. apply or_dec; try apply updater_thread_dec.
+      apply and_dec; try apply updater_thread_dec.
+      apply neg_seq_spec_dec. }
       
     destruct (decide (updater_thread op vp = true 
       ∨ (updater_thread op vp = false 
           ∧ ¬ seq_spec op (abs (M0 !!! T0)) (abs (M0 !!! T0)) vp))) 
-      as [Hcase1 | Hcase2].
+      as [Hcase1 | Hcase2]; clear Hdec.
     - iMod (inv_alloc (threadN N) _
               (∃ M T, State γ_sy γ_tk (au N γ_s op Φ) Φ M T op vp T0) 
                                     with "[AU Hc Hreg_sy1]") as "#HthInv".
@@ -345,7 +345,7 @@ Section counter.
           assert (t = T0) as -> by lia. contradiction. }
 
       iModIntro. iSplitR "Hproph Token". iNext.
-      iExists M0, T0, n0. iFrame "∗%".
+      iExists M0, T0, s0. iFrame "∗%".
       iExists (R ∪ {[tid]}), hγt'. iFrame.
       iSplitR. iPureIntro. subst hγt'.
       apply leibniz_equiv. rewrite dom_insert.
@@ -357,31 +357,27 @@ Section counter.
                   by (clear -tid_notin_R; set_solver).
       by rewrite H'.
       
-      iModIntro. wp_bind (counterOp _ _ _)%E.
+      iModIntro. wp_bind (dsOp _ _)%E.
       
       iAssert (update_helping_protocol N γ_t γ_s γ_td γ_ght)%I as "Upd_help".
       { admit. }
       iAssert (thread_vars γ_t γ_ght γ_sy tid T0)%I as "#Thr_vars".
       { iFrame "#". }
       
-      wp_apply counterOp_spec; try done.
-      (*
-      iAaccIntro with ""; try done.
-      { iIntros "_"; iModIntro; eauto with iFrame. }
-      iIntros (res)"HpastW". iModIntro.
-      *)
+      wp_apply dsOp_spec; try done.
       iIntros (res)"HpastW".
       wp_pures.
-      wp_apply (typed_proph_wp_resolve1 NatTypedProph with "Hproph");
-         try done.
-      wp_pures. iModIntro. iIntros "%vp_eqZ_res".
-      assert (vp = res) as vp_eq_res by (clear -vp_eqZ_res; lia).
-      clear vp_eqZ_res. subst vp.
+      wp_apply ((typed_proph_wp_resolve1 resTTypedProph 
+                  _ _ _ _ _ _ _ (res))
+        with "Hproph"); try done.
+      { unfold typed_proph_from_val. simpl.
+        apply resT_proph_resolve. }  
+      wp_pures. iModIntro. iIntros "%vp_eq_res". subst vp.
        
       iApply fupd_wp.
       
       iInv "HthInv" as (M1_th T1_th)"(>Hth_sy & >% & Hth_or)".
-      iInv "HInv" as (M1 T1 n1) "(>HCntr & >%Habs1 & >Hist & Help & Templ)".
+      iInv "HInv" as (M1 T1 s1) "(>HCntr & >%Habs1 & >Hist & Help & Templ)".
       iDestruct "Help" as (R1 hγt1)"(>HR & >Hγt 
                                   & >Domm_hγt & Hstar_reg)".
       
@@ -398,12 +394,11 @@ Section counter.
                ∗ ([∗ set] t_id ∈ R1, Reg N γ_t γ_s γ_ght t_id M1)
                ∗ own (γ_sy) (to_frac_agree (1 / 2) M1_th) ))%I
                 with "[Hstar_reg Hth_sy]" as "(>% & >% & Hstar_reg & >Hth_sy)". 
-      { admit.
-        (*
+      { 
         iEval (rewrite (big_sepS_elem_of_acc _ (R1) tid); 
                                 last by eauto) in "Hstar_reg".
         iDestruct "Hstar_reg" as "(Hreg_t & Hstar_reg')".
-        iDestruct "Hreg_t" as (P Q γ_tk' γ_sy' t0 vp' vtid')
+        iDestruct "Hreg_t" as (γ_tk' γ_sy' Q' op' vp' t0' vtid')
                           "(Hreg_proph & >Hreg_gh' & >Hreg_sy & Ht_reg')".
 
         iDestruct "Hreg_gh'" as "(Hreg_gh' & #?)".
@@ -416,28 +411,32 @@ Section counter.
         apply leibniz_equiv in Valid.
         injection Valid; intros <- <-.
                   
-        iAssert (⌜M1_th = M1⌝)%I as "%".
+        iAssert (⌜M1_th = M1 ∧ T1_th = T1⌝)%I as "(% & %)".
         { iPoseProof (own_valid_2 _ _ _ with "[$Hth_sy] [$Hreg_sy]") 
               as "V_M".
           iDestruct "V_M" as %V_M.
           apply frac_agree_op_valid in V_M. destruct V_M as [_ V_M].
-          apply leibniz_equiv_iff in V_M.
-          by iPureIntro. } subst M1_th.
+          iPureIntro. split; first by apply leibniz_equiv. admit. } 
+        subst M1_th T1_th.
+          
+        iSplitR. { by iPureIntro. } 
         iSplitR. iNext; by iPureIntro.
         iSplitR "Hth_sy". iApply "Hstar_reg'".
-        iNext. iExists P, Q, γ_tk', γ_sy, T0, vp', vtid'.
+        iNext. iExists γ_tk', γ_sy, Q', op', vp', T0, vtid'.
         iFrame "∗#". by iNext. 
-        *)
       } subst M1_th T1_th.
       
       iEval (unfold past_lin_witness) in "HpastW".
       (* iEval (rewrite Upd_thr) in "HpastW".*)
 
       iDestruct "Hth_or" as "[Hth_or | Hth_or]".
-      { iDestruct "Hth_or" as "(AU & Hc & >%)".
-        rename H into HPending.
-        exfalso. apply HPending.
-        admit. }  
+      { iDestruct "Hth_or" as "(AU & Hc & >%HPending)".
+        destruct (decide (updater_thread op res = true))
+          as [Hdec | Hdec]. 
+        - rewrite Hdec. rewrite Hdec in HPending.
+          iExFalso. admit. 
+        - destruct (decide (updater_thread op res = false)) as [Hdec' | Hdec']; try done. 
+          rewrite Hdec'. rewrite Hdec' in HPending. admit. }  
       
       iDestruct "Hth_or" as "(Hth_or & Hpast)".  
       iDestruct "Hth_or" as "[Hth_or | >Hth_or]"; last first.
@@ -445,7 +444,7 @@ Section counter.
         exfalso; try done. }
         
       iModIntro. iSplitR "Hth_or Hth_sy Token Hpast".
-      iExists M1, T1, n1; iFrame "∗%".
+      iExists M1, T1, s1; iFrame "∗%".
       iNext. iExists R1, hγt1; iFrame.     
 
       iModIntro. iSplitL "Token Hth_sy Hpast".
@@ -460,60 +459,57 @@ Section counter.
         - exfalso; apply Hcase2. left; try done.
         - exfalso; apply Hcase2. left; try done. 
         - done. 
-        - destruct (decide (seq_spec op (abs (M0 !!! T0)) (abs (M0 !!! T0)) vp));
+        - assert (Decision (seq_spec op (abs (M0 !!! T0)) (abs (M0 !!! T0)) vp)) as H'.
+          { apply seq_spec_dec. }
+          destruct (decide (seq_spec op (abs (M0 !!! T0)) (abs (M0 !!! T0)) vp));
             try done. 
           exfalso. apply Hcase2. right.
           split; try done. } 
-      iMod "AU" as (n) "[Cntr [_ Hcomm]]".
-        iAssert (⌜n = n0⌝)%I as "%". { admit. } subst n. 
-        iSpecialize ("Hcomm" $! n0 vp). 
-        iMod ("Hcomm" with "[Cntr]") as "HΦ".
-        { iFrame. rewrite Habs0 in Hss. by iPureIntro. }
+      iMod "AU" as (c) "[Cntr [_ Hcomm]]".
+      iAssert (⌜c = abs s0⌝)%I as "%". { admit. } subst c. 
+      iSpecialize ("Hcomm" $! (abs s0) vp). 
+      iMod ("Hcomm" with "[Cntr]") as "HΦ".
+      { iFrame. rewrite Habs0 in Hss. by iPureIntro. }
+   
+      iAssert (past_lin M0 T0 op vp T0)%I as "Hpast".
+      { iPureIntro. rewrite Upd_thr. exists T0.
+        split; try done. }
         
-        iAssert (past_lin M0 T0 op vp T0)%I as "Hpast".
-        { iPureIntro. rewrite Upd_thr. exists T0.
-          split; try done. }
-        
-        iMod (inv_alloc (threadN N) _
-              (∃ M T, State γ_sy γ_tk (au N γ_s op Φ) Φ M T op vp T0) 
-                                    with "[Hreg_sy1 Token]") as "#HthInv".
-        { iNext. iExists M0, T0. iFrame "Hreg_sy1".
-          iSplitR. by iPureIntro.
-          iRight. unfold Done. iFrame "Hpast".
-          by iRight. }
-        
-        iAssert (update_helping_protocol N γ_t γ_s γ_td γ_ght)%I as "Upd_help".
-        { admit. }
-        iAssert (thread_vars γ_t γ_ght γ_sy tid T0)%I as "#Thr_vars".
-        { iFrame "#". }
+      iMod (inv_alloc (threadN N) _
+            (∃ M T, State γ_sy γ_tk (au N γ_s op Φ) Φ M T op vp T0) 
+                                  with "[Hreg_sy1 Token]") as "#HthInv".
+      { iNext. iExists M0, T0. iFrame "Hreg_sy1".
+        iSplitR. by iPureIntro.
+        iRight. unfold Done. iFrame "Hpast".
+        by iRight. }
+      
+      iAssert (update_helping_protocol N γ_t γ_s γ_td γ_ght)%I as "Upd_help".
+      { admit. }
+      iAssert (thread_vars γ_t γ_ght γ_sy tid T0)%I as "#Thr_vars".
+      { iFrame "#". }
   
       
-        iModIntro. iSplitR "Hproph HΦ". iNext.
-        iExists M0, T0, n0.  iFrame "∗%".
-        iExists (R ∪ {[tid]}), hγt'. iFrame.
-        iSplitR. iPureIntro. subst hγt'.
-        apply leibniz_equiv. rewrite dom_insert.
-        rewrite Domm_hγt. clear; set_solver.
-        rewrite (big_sepS_delete _ (R ∪ {[tid]}) tid); last by set_solver.
-        iSplitR "Hstar_reg". unfold Reg.
-        iExists γ_tk, γ_sy, Φ, op, vp, T0, vtid. iFrame "∗#".
-        assert ((R ∪ {[tid]}) ∖ {[tid]} = R) as H' 
-                  by (clear -tid_notin_R; set_solver).
-        by rewrite H'.  
+      iModIntro. iSplitR "Hproph HΦ". iNext.
+      iExists M0, T0, s0.  iFrame "∗%".
+      iExists (R ∪ {[tid]}), hγt'. iFrame.
+      iSplitR. iPureIntro. subst hγt'.
+      apply leibniz_equiv. rewrite dom_insert.
+      rewrite Domm_hγt. clear; set_solver.
+      rewrite (big_sepS_delete _ (R ∪ {[tid]}) tid); last by set_solver.
+      iSplitR "Hstar_reg". unfold Reg.
+      iExists γ_tk, γ_sy, Φ, op, vp, T0, vtid. iFrame "∗#".
+      assert ((R ∪ {[tid]}) ∖ {[tid]} = R) as H' 
+                by (clear -tid_notin_R; set_solver).
+      by rewrite H'.  
         
-        iModIntro.
-        (*
-        awp_apply counterOp_spec without "HΦ"; try done.
-        iAaccIntro with ""; try done.
-        { iIntros "_". iModIntro; try eauto with iFrame. } 
-        iIntros (res) "HpastW". 
-        iModIntro. iIntros "HΦ". wp_pures.
-        *)
-        wp_apply counterOp_spec; try done.
-        iIntros (res)"HpastW". wp_pures.
-        wp_apply (typed_proph_wp_resolve1 NatTypedProph with "Hproph"); 
-          try done.
-        wp_pures. iModIntro. iIntros "%". rename H into vp_eq_res. 
-        assert (vp = res). { clear -vp_eq_res. lia. } 
-        clear vp_eq_res. wp_pures. iModIntro. by subst vp.
+      iModIntro.
+      wp_apply dsOp_spec; try done.
+      iIntros (res)"HpastW". wp_pures.
+      wp_apply ((typed_proph_wp_resolve1 resTTypedProph 
+                  _ _ _ _ _ _ _ (res))
+        with "Hproph"); try done.
+      { unfold typed_proph_from_val. simpl.
+        apply resT_proph_resolve. }  
+      wp_pures. iModIntro. iIntros "->".
+      wp_pures. iModIntro. done. 
   Admitted.  
